examples/miniML/metatheory/evaluateEquationsScript.sml
@@ -16,6 +16,8 @@ val evaluate_val = Q.store_thm(
   (evaluate cenv env (Val v) r = (r = Rval v))`,
 rw [Once evaluate_cases]);
 
+val _ = export_rewrites["evaluate_raise","evaluate_val"];
+
 val evaluate_con = Q.store_thm(
 "evaluate_con",
 `!cenv env cn es r.
@@ -27,6 +29,76 @@ val evaluate_con = Q.store_thm(
            (r = Rval (Conv cn vs)))
    else (r = Rerr Rtype_error))`,
 rw [Once evaluate_cases] >>
+metis_tac []);
+
+val evaluate'_raise = store_thm(
+"evaluate'_raise",
+``∀env err r. evaluate' env (Raise err) r = (r = Rerr (Rraise err))``,
+rw [Once evaluate'_cases])
+
+val evaluate'_val = store_thm(
+"evaluate'_val",
+``∀env v r. evaluate' env (Val v) r = (r = Rval v)``,
+rw [Once evaluate'_cases])
+
+val evaluate'_fun = store_thm(
+"evaluate'_fun",
+``∀env n e r. evaluate' env (Fun n e) r = (r = Rval (Closure env n e))``,
+rw [Once evaluate'_cases])
+
+val _ = export_rewrites["evaluate'_raise","evaluate'_val","evaluate'_fun"]
+
+val evaluate'_con = store_thm(
+"evaluate'_con",
+``∀env cn es r. evaluate' env (Con cn es) r =
+  (∃err. evaluate_list' env es (Rerr err) ∧ (r = Rerr err)) ∨
+  (∃vs. evaluate_list' env es (Rval vs) ∧ (r = Rval (Conv cn vs)))``,
+rw [Once evaluate'_cases] >>
+metis_tac [])
+
+val evaluate'_var = store_thm(
+"evaluate'_var",
+``∀env n r. evaluate' env (Var n) r =
+  (∃v. (lookup n env = SOME v) ∧ (r = Rval v)) ∨
+  ((lookup n env = NONE) ∧ (r = Rerr Rtype_error))``,
+rw [Once evaluate'_cases] >>
+metis_tac [])
+
+val evaluate_list'_thm = store_thm(
+"evaluate_list'_thm",
+``∀env r.
+  (evaluate_list' env [] r = (r = Rval [])) ∧
+  (∀e es. evaluate_list' env (e::es) r =
+   (∃v vs. evaluate' env e (Rval v) ∧ evaluate_list' env es (Rval vs) ∧
+           (r = Rval (v::vs))) ∨
+   (∃err. evaluate' env e (Rerr err) ∧
+          (r = Rerr err)) ∨
+   (∃v err. evaluate' env e (Rval v) ∧ evaluate_list' env es (Rerr err) ∧
+            (r = Rerr err)))``,
+rw[] >-
+  rw[Once evaluate'_cases] >>
+rw[EQ_IMP_THM] >- (
+  pop_assum (mp_tac o (SIMP_RULE (srw_ss()) [Once evaluate'_cases])) >>
+  rw [] >> metis_tac[] )
+>- rw [evaluate'_rules]
+>- rw [evaluate'_rules] >>
+rw[Once evaluate'_cases] >>
+metis_tac [])
+
+val evaluate'_app = store_thm(
+"evaluate'_app",
+``∀env op e1 e2 r. evaluate' env (App op e1 e2) r =
+  (∃v1 v2 env' e. evaluate' env e1 (Rval v1) ∧ (evaluate' env e2 (Rval v2)) ∧
+                  (do_app env op v1 v2 = SOME (env',e)) ∧
+                  evaluate' env' e r) ∨
+  (∃v1 v2. evaluate' env e1 (Rval v1) ∧ (evaluate' env e2 (Rval v2)) ∧
+           (do_app env op v1 v2 = NONE) ∧
+           (r = Rerr Rtype_error)) ∨
+  (∃v1 err. evaluate' env e1 (Rval v1) ∧ (evaluate' env e2 (Rerr err)) ∧
+            (r = Rerr err)) ∨
+  (∃err. evaluate' env e1 (Rerr err) ∧
+         (r = Rerr err))``,
+rw[Once evaluate'_cases] >>
 metis_tac []);
 
 val _ = export_theory ()
